src/Linearizable2.v
@@ -1,6 +1,5 @@
 Require Import Mem.
 Require Import Pred.
-Require Import Locking.
 Require Import EventCSL.
 Require Import FunctionalExtensionality.
 Require Import Automation.
@@ -253,139 +252,38 @@ Arguments linear_mem {A AEQ V}.
     autorewrite with upd; auto.
   Qed.
 
-Definition linearized_consistent A AEQ V (m: @linear_mem A AEQ V) (locks: _ -> BusyFlagOwner) : Prop :=
-forall a, match m a with
-          | Some (v, v') =>
-            match locks a with
-            | Owned _ => True
-            | NoOwner => v = v'
-            end
-          | None => True
-          end.
+  Definition linear_upd A AEQ V (m: @linear_mem A AEQ V) a v :=
+    match m a with
+    | Some (v0, _) => upd m a (v0, v)
+    | None => m
+    end.
 
-Definition linear_rel A AEQ V tid (locks locks': A -> BusyFlagOwner)
-  (m m': @linear_mem A AEQ V) :=
-  (* lock protocol *)
-  (forall a, lock_transition tid (locks a) (locks' a)) /\
-  (* lock protection *)
-  (forall a tid', locks a = Owned tid' ->
-  tid <> tid' ->
-  m' a = m a).
+  Theorem linear_upd_eq : forall A AEQ V (m: @linear_mem A AEQ V) a v0 v0' v,
+      m a = Some (v0, v0') ->
+      linear_upd m a v a = Some (v0, v).
+  Proof.
+    unfold linear_upd; intros; simpl_match;
+    autorewrite with upd; auto.
+  Qed.
 
-Theorem linear_rel_refl : forall A AEQ V tid locks (m: @linear_mem A AEQ V),
-  linear_rel tid locks locks m m.
-Proof.
-  unfold linear_rel; intuition.
-Qed.
+  Theorem linear_upd_view_eq : forall A AEQ V (m: @linear_mem A AEQ V) a v0 v,
+      view LinPoint m a = Some v0 ->
+      linear_upd m a v a = Some (v0, v).
+  Proof.
+    unfold view, proj, linear_upd; intros;
+    destruct matches; subst;
+    cbn in *;
+    autorewrite with upd;
+    repeat simpl_match;
+    try congruence.
+    inversion H; auto.
+  Qed.
 
-Theorem linear_rel_trans : forall A AEQ V tid locks locks' locks''
-  (m m' m'': @linear_mem A AEQ V),
-  linear_rel tid locks locks' m m' ->
-  linear_rel tid locks' locks'' m' m'' ->
-  linear_rel tid locks locks'' m m''.
-Proof.
-  unfold linear_rel; intros; intuition;
-    specialize_all A.
-  - eapply lock_transition_trans; eauto.
-
-  - eapply eq_trans with (y := m' a); eauto.
-    inversion H1; subst; try intuition congruence.
-    eapply (H3 tid'); (congruence || eauto).
-Qed.
-
-Definition linear_upd A AEQ V (m: @linear_mem A AEQ V) a v :=
-  match m a with
-  | Some (v0, _) => upd m a (v0, v)
-  | None => m
-  end.
-
-Theorem linear_upd_eq : forall A AEQ V (m: @linear_mem A AEQ V) a v0 v0' v,
-    m a = Some (v0, v0') ->
-    linear_upd m a v a = Some (v0, v).
-Proof.
-  unfold linear_upd; intros; simpl_match;
-  autorewrite with upd; auto.
-Qed.
-
-Theorem linear_upd_view_eq : forall A AEQ V (m: @linear_mem A AEQ V) a v0 v,
-    view LinPoint m a = Some v0 ->
-    linear_upd m a v a = Some (v0, v).
-Proof.
-  unfold view, proj, linear_upd; intros;
-  destruct matches; subst;
-  cbn in *;
-  autorewrite with upd;
-  repeat simpl_match;
-  try congruence.
-  inversion H; auto.
-Qed.
-
-Theorem linear_upd_neq : forall A AEQ V (m: @linear_mem A AEQ V) a a' v,
-    a <> a' ->
-    linear_upd m a v a' = m a'.
-Proof.
-  unfold linear_upd; intros;
-  destruct matches;
-  autorewrite with upd; auto.
-Qed.
-
-Theorem linearized_consistent_upd : forall A AEQ V (m: @linear_mem A AEQ V)
-  locks a tid v,
-  locks a = Owned tid ->
-  linearized_consistent m locks ->
-  linearized_consistent (linear_upd m a v) locks.
-Proof.
-  unfold linearized_consistent, linear_upd; intros;
-    learn_all A.
-  destruct matches;
-  destruct (AEQ a a0); subst;
-    autorewrite with upd in *;
-    cleanup.
-Qed.
-
-Theorem linearized_consistent_release : forall A AEQ V (m: @linear_mem A AEQ V)
-  locks a,
-  linearized_consistent m locks ->
-  locks a = NoOwner ->
-  linearized_consistent (lin_release m a) locks.
-Proof.
-  unfold linearized_consistent, lin_release; intros.
-  specialize_all A.
-  destruct matches;
-  destruct (AEQ a a0); subst;
-  autorewrite with upd in *;
-  cleanup.
-Qed.
-
-Hint Rewrite lin_release_eq linear_upd_eq using (solve [ auto ] ) : lin_upd.
-Hint Rewrite lin_release_view_eq linear_upd_view_eq using (solve [ auto ] ) : lin_upd.
-Hint Rewrite lin_release_neq linear_upd_neq using (solve [ auto ] ) : lin_upd.
-
-Theorem linear_rel_upd :
-  forall tid A AEQ V
-    locks locks' (m m': @linear_mem A AEQ V)
-    a v,
-    locks a = Owned tid ->
-    linear_rel tid locks locks' m m' ->
-    linear_rel tid locks locks'
-               m (linear_upd m' a v).
-Proof.
-  unfold linear_rel, linear_upd; intuition.
-  destruct (AEQ a a0); try congruence.
-  destruct matches; autorewrite with upd; eauto.
-Qed.
-
-Lemma linear_upd_same_domain : forall A AEQ V (m: @linear_mem A AEQ V) a v',
-    same_domain m (linear_upd m a v').
-Proof.
-  unfold same_domain, subset, linear_upd; intuition.
-  destruct (AEQ a a0); subst; intros;
-  destruct matches;
-  autorewrite with upd;
-  eauto.
-
-  destruct (AEQ a a0); subst; intros;
-  destruct matches in *;
-  autorewrite with upd in *;
-  eauto.
-Qed.
+  Theorem linear_upd_neq : forall A AEQ V (m: @linear_mem A AEQ V) a a' v,
+      a <> a' ->
+      linear_upd m a v a' = m a'.
+  Proof.
+    unfold linear_upd; intros;
+    destruct matches;
+    autorewrite with upd; auto.
+  Qed.
